compiler/backend/proofs/README.md
@@ -14,7 +14,7 @@ Correctness proof for bvi_let
 Correctness proof for bvi_tailrec
 
 [bvi_tmcProofScript.sml](bvi_tmcProofScript.sml):
-Correctness proof for bvi_tmc
+Correctness proof for bvi_tailrec
 
 [bvi_to_dataProofScript.sml](bvi_to_dataProofScript.sml):
 Correctness proof for bvi_to_data
